MirrorCharge!/src/MirrorCharge/Java/Syntax.v
@@ -1,5 +1,6 @@
 Require Import Java.Language.Lang.
 Require Import Java.Logic.AssertionLogic.
+Require Import Coq.Strings.String.
 
 Require Import ExtLib.Core.RelDec.
 Require Import ExtLib.Data.String.
@@ -8,23 +9,51 @@ Require Import MirrorCore.TypesI.
 Require Import MirrorCore.Lambda.Expr.
 Require MirrorCore.syms.SymEnv.
 Require MirrorCore.syms.SymSum.
-Require Import MirrorCore.Subst.FMapSubst3.
+Require Import MirrorCore.Subst.FMapSubst.
 Require Import MirrorCore.Lambda.ExprSubst.
 Require Import MirrorCore.Lambda.ExprUnify_simul.
 Require Import MirrorCharge.ILogicFunc.
+Require Import ExtLib.Structures.Applicative.
+
+Require Import Charge.Open.Stack.
+
+Require Import Java.Logic.SpecLogic.
+Require Import Java.Logic.AssertionLogic.
+Require Import Java.Semantics.OperationalSemantics.
+Require Import Java.Language.Program.
+Require Import Java.Language.Lang.
 
 Set Implicit Arguments.
 Set Strict Implicit.
 
+Local Instance Applicative_Fun A : Applicative (Fun A) :=
+{ pure := fun _ x _ => x
+; ap := fun _ _ f x y => (f y) (x y)
+}.
+
 Inductive typ :=
 | tyArr : typ -> typ -> typ
-| tyList : typ -> typ
+| tyVarList : typ
 | tyVar : typ
-| tyProp : typ.
+| tyVal : typ
+| tyString : typ
+| tyProp : typ
+| tySpec : typ
+| tyAsn : typ
+| tyProg : typ
+| tyStack : typ
+| tyCmd : typ.
+
+Notation "'tyPure'" := (tyArr tyStack tyProp).
+Notation "'tySasn'" := (tyArr tyStack tyAsn). 
 
 Fixpoint type_cast_typ (a b : typ) : option (a = b) :=
   match a as a , b as b return option (a = b) with
     | tyProp , tyProp => Some eq_refl
+    | tySpec , tySpec => Some eq_refl
+    | tyVal, tyVal => Some eq_refl
+    | tyProg, tyProg => Some eq_refl
+    | tyVarList, tyVarList => Some eq_refl
     | tyArr x y , tyArr a b =>
       match type_cast_typ x a , type_cast_typ y b with
         | Some pf , Some pf' =>
@@ -37,15 +66,9 @@ Fixpoint type_cast_typ (a b : typ) : option (a = b) :=
         | _ , _ => None
       end
     | tyVar , tyVar => Some eq_refl
-    | tyList t, tyList u =>
-    	match type_cast_typ t u with
-    		| Some pf => 
-    		  Some (match pf in _ = a return tyList t = tyList a with
-    			| eq_refl => eq_refl
-    		  end)
-    		| None => None
-        end
-    | _ , _ => None
+    | tyString, tyString => Some eq_refl
+    | tyCmd, tyCmd => Some eq_refl
+    | _, _ => None
   end.
 
 Instance RelDec_eq_typ : RelDec (@eq typ) :=
@@ -58,14 +81,20 @@ Fixpoint typD (ls : list Type) (t : typ) : Type :=
   match t with
     | tyArr a b => typD ls a -> typD ls b
     | tyProp => Prop
-    | tyList a => list (typD ls a)
-    | tyVar => var
+    | tySpec => spec
+    | tyAsn => asn
+    | tyVarList => list Lang.var 
+    | tyVar => Lang.var
+    | tyVal => sval
+    | tyString => string
+    | tyProg => Prog_wf
+    | tyStack => stack
+    | tyCmd => cmd
   end.
   
 Inductive tyAcc_typ : typ -> typ -> Prop :=
 | tyAcc_tyArrL : forall a b, tyAcc_typ a (tyArr a b)
 | tyAcc_tyArrR : forall a b, tyAcc_typ a (tyArr b a).
-
 
 Instance RType_typ : RType typ :=
 { typD := typD
@@ -94,33 +123,63 @@ Instance Typ0_Prop : Typ0 _ Prop :=
 }.
 
 Inductive java_func :=
-| pVar (_ : var)
+| pVar (_ : Lang.var)
+| pString (_ : string)
+| pVal (_ : sval)
+| pVarList (_ : list Lang.var)
+| pProg (_ : Prog_wf)
+| pCmd (_ : cmd)
 | pEq (_ : typ)
-| pNil (_ : typ)
-| pCons (_ : typ)
-| pAp (_ _ : typ).
 
+| pAp (_ _ : typ)
+| pApConst (_ : typ)
+| pMethodSpec
+| pProgEq
+| pTriple
+
+| pStackGet
+| pStackSet.
 
 Definition func := (SymEnv.func + java_func + ilfunc typ)%type.
 
 Definition typeof_sym_java (f : java_func) : option typ :=
   match f with
     | pVar _ => Some tyVar
-    | pNil t => Some (tyList t)
+    | pString _ => Some tyString
+    | pVal _ => Some tyVal
+    | pProg _ => Some tyProg
+    | pVarList _ => Some tyVarList
+    | pCmd _ => Some tyCmd
     | pEq t => Some (tyArr t (tyArr t tyProp))
-    | pCons t => Some (tyArr t (tyArr (tyList t) (tyList t)))
-    | pAp t u => Some (tyArr (tyArr t u) (tyArr t u))
-  end.
+    | pAp t u => Some (tyArr (tyArr tyStack (tyArr t u)) (tyArr (tyArr tyStack t) (tyArr tyStack u)))
+    | pApConst t => Some (tyArr t (tyArr tyStack t))
+    | pMethodSpec => Some (tyArr tyString (tyArr tyString (tyArr tyVarList
+    	 (tyArr tyVar (tyArr tySasn (tyArr tySasn tySpec))))))
+    | pProgEq => Some (tyArr tyProg tySpec)
+    | pStackGet => Some (tyArr tyVar (tyArr tyStack tyVal))
+    | pStackSet => Some (tyArr tyVar (tyArr tyVal (tyArr tyStack tyStack)))
+    | pTriple => Some (tyArr tySasn (tyArr tySasn (tyArr tyCmd tySpec)))
+    end.
   
 Definition java_func_eq (a b : java_func) : option bool :=
   match a , b with
     | pVar a , pVar b => Some (a ?[ eq ] b)
+    | pVarList a, pVarList b => Some (a ?[ eq ] b)
+    | pString a, pString b => Some (a ?[ eq ] b)
+    | pCmd a, pCmd b => Some true (* THIS IS FALSE! Syntactic equality on commands is required *)
+    | pProg a, pProg b => Some true (* THIS IS FALSE! We need an equivalence checker for programs. This should just be syntactic equality. *)
     | pEq a , pEq b => Some (a ?[ eq ] b)
-    | pNil t , pNil u => Some (t ?[ eq ] u)
-    | pCons t , pCons u => Some (t ?[ eq ] u) 
+        
     | pAp t u , pAp t' u' => Some (t ?[ eq ] t' && u ?[ eq ] u')%bool
+    | pApConst t, pApConst u => Some (t ?[ eq ] u)
+    | pMethodSpec, pMethodSpec => Some true
+    | pProgEq, pProgEq => Some true
+    | pStackGet, pStackGet => Some true
+    | pStackSet, pStackSet => Some true
+    | pTriple, pTriple => Some true
     | _, _ => None
   end.
+
 
 Instance RSym_imp_func : SymI.RSym java_func :=
 { typeof_sym := typeof_sym_java
@@ -131,20 +190,36 @@ Instance RSym_imp_func : SymI.RSym java_func :=
                                 end
             with
               | pVar v => v
+              | pString s => s
+              | pProg p => p
+              | pVal v => v
+              | pVarList lst => lst
+              | pCmd c => c
               | pEq t => @eq (typD ts t)
-              | pNil t => @nil (typD ts t)
-              | pCons t => @cons (typD ts t)
-              | pAp t u => fun g a => g a
+              
+              | pAp t u => @Applicative.ap (Fun stack) (Applicative_Fun _) (typD ts t) (typD ts u)
+              | pApConst t => @Applicative.pure (Fun stack) (Applicative_Fun _) (typD ts t)
+              | pMethodSpec => method_spec
+              | pProgEq => prog_eq
+              | pStackGet => fun x s => s x
+              | pStackSet => stack_add
+              
+              | pTriple => triple
             end
 ; sym_eqb := java_func_eq
 }.
 
+Require Import Charge.Logics.ILInsts.
+
+Local Existing Instance ILFun_Ops.
+Local Existing Instance ILFun_ILogic.
+
 Definition fs : @SymEnv.functions typ _ :=
   SymEnv.from_list
-    (@SymEnv.F typ _ (tyArr tyVar (tyArr (tyList tyVar)  tyProp))
-               (fun _ => (@In var)) ::
-     @SymEnv.F typ _ (tyArr (tyList tyVar) tyProp)
-               (fun _ => (@NoDup var)) ::
+    (@SymEnv.F typ _ (tyArr tyVar (tyArr tyVarList  tyProp))
+               (fun _ => (@In (Lang.var))) ::
+     @SymEnv.F typ _ (tyArr tyVarList tyProp)
+               (fun _ => (@NoDup (Lang.var))) ::
      nil).
      
 Definition lops : logic_ops _ :=
@@ -153,6 +228,10 @@ Definition lops : logic_ops _ :=
           return option (forall ts, ILogic.ILogicOps (TypesI.typD ts t))
     with
       | tyProp => Some _
+      | tyAsn => Some _
+      | tySasn => Some (fun _ => @ILFun_Ops stack asn _)
+      | tySpec => Some _
+      | tyPure => Some (fun _ => @ILFun_Ops stack Prop _)
       | _ => None
     end.
 
@@ -166,16 +245,6 @@ Definition eops : embed_ops _ :=
       | _ , _ => None
     end.
 
-Definition subst : Type :=
-  FMapSubst3.SUBST.raw (expr typ func).
-Definition SS : SubstI3.Subst subst (expr typ func) :=
-  @FMapSubst3.SUBST.Subst_subst _.
-Definition SU : SubstI3.SubstUpdate subst (expr typ func) :=
-  @FMapSubst3.SUBST.SubstUpdate_subst (expr typ func)
-                                      (@mentionsU typ func)
-                                      (@instantiate typ func).
-
-
 Local Instance RSym_ilfunc : SymI.RSym (ilfunc typ) :=
   @ILogicFunc.RSym_ilfunc typ _ _ lops eops _ _.
 
@@ -183,37 +252,66 @@ Definition RS : SymI.RSym func :=
   SymSum.RSym_sum (SymSum.RSym_sum (SymEnv.RSym_func fs) _) _.
 Local Existing Instance RS.
 
+Instance RTypeOk_typ : @RTypeOk _ RType_typ.
+Proof.
+	admit.
+Qed.
+
+Instance Typ2Ok_typ : Typ2Ok Typ2_Fun.
+Proof.
+	admit.
+Qed.
+
+Instance RSym_ok : SymI.RSymOk RS.
+Proof.
+	admit.
+Qed.
+
 Let Expr_expr : ExprI.Expr _ (expr typ func) := Expr_expr _ _.
+Let Expr_ok : @ExprI.ExprOk typ RType_typ (expr typ func) Expr_expr := ExprOk_expr nil.
 Local Existing Instance Expr_expr.
+Local Existing Instance Expr_ok.
 
-Definition fVar (v : var) : expr typ func := Inj (inl (inr (pVar v))).
-Definition fIn : expr typ func := Inj (inl (inl 1%positive)).
-Definition fNoDup : expr typ func := Inj (inl (inl 2%positive)).
-Definition fAp (t u : typ) : expr typ func := Inj (inl (inr (pAp t u))).
-Definition fNil t : expr typ func := Inj (inl (inr (pNil t))).
-Definition fCons t : expr typ func := Inj (inl (inr (pCons t))).
+Definition subst : Type :=
+  FMapSubst.SUBST.raw (expr typ func).
+Definition SS : SubstI.Subst subst (expr typ func) :=
+  @FMapSubst.SUBST.Subst_subst _.
+Definition SU : SubstI.SubstUpdate subst (expr typ func) :=
+  FMapSubst.SUBST.SubstUpdate_subst (@instantiate typ func).
+Definition SO : SubstI.SubstOk Expr_expr SS := 
+  @FMapSubst.SUBST.SubstOk_subst typ RType_typ (expr typ func) _ _.
 
-Definition leq (t : typ) : expr typ func := Inj (inl (inr (pEq t))).
-Definition lap (t u : typ) (a b : expr typ func) : expr typ func :=
-  App (App (fAp t u) a) b.
-Definition mkCons (t : typ) (x xs : expr typ func) :=
-  App (App (fCons t) x) xs.
-(*  lap (tyList t) (tyList t) (lap t (tyArr (tyList t) (tyList t)) (fCons t) x) xs.*)
-Definition mkIn (x lst : expr typ func) :=
-  App (App fIn x) lst.
-(*  lap (tyList tyVar) tyProp (lap tyVar (tyArr (tyList tyVar) tyProp) fIn x) lst.*)
-Definition mkNoDup (lst : expr typ func) :=
-  App fNoDup lst.
+Local Existing Instance SS.
+Local Existing Instance SU.
+Local Existing Instance SO.
 
+Notation "'fMethodSpec'" := (Inj (inl (inr pMethodSpec))) (at level 0).
+Notation "'fProgEq'" := (Inj (inl (inr pProgEq))) (at level 0).
+Notation "'fTriple'" := (Inj (inl (inr pTriple))) (at level 0).
 
+Notation "'fEq' t" := (Inj (inl (inr (pEq t)))) (at level 0).
+Notation "'fAp'" := (Inj (inl (inr pAp))) (at level 0).
+
+Notation "'mkAp' t u a b" := (App (App (fAp t u) a) b) (at level 0).
+Notation "'mkMethodSpec' '[' C ',' m ',' args ',' r ',' p ',' q ']'" := 
+    (App (App (App (App (App (App fMethodSpec C) m) args) r) p) q) (at level 0).
+Notation "'mkTriple' '[' P ',' c ',' Q ']'" := (App (App (App fTriple P) c) Q) (at level 0).
+	
+Notation "'mkVar' '[' x ']'" := (Inj (inl (inr (pVar x)))) (at level 0).
+Notation "'mkVal' '[' v ']'" := (Inj (inl (inr (pVal v)))) (at level 0).
+Notation "'mkVarList' '[' lst ']'" := (Inj (inl (inr (pVarList lst)))) (at level 0).
+Notation "'mkString' '[' s ']'" := (Inj (inl (inr (pString s)))) (at level 0).
+Notation "'mkProg' '[' P ']'" := (Inj (inl (inr (pProg P)))) (at level 0).
+Notation "'mkProgEq' '[' P ']'" := (App fProgEq P) (at level 0).
+Notation "'mkCmd' '[' c ']'" := (Inj (inl (inr (pCmd c)))) (at level 0).
+	
 Definition land (l : typ) (e e' : expr typ func) : expr typ func :=
   App (App (Inj (inr (ilf_and l))) e) e'.
 Definition ltrue (l : typ) : expr typ func :=
   Inj (inr (ilf_true l)).
 Definition lfalse (l : typ) : expr typ func :=
   Inj (inr (ilf_false l)).
-Definition lentails (l : typ) (e e' : expr typ func) : expr typ func :=
-  App (App (Inj (inr (ilf_entails l))) e) e'.
+Notation "'mkEntails' '[' l ',' e ',' e' ']'" := (App (App (Inj (inr (ilf_entails l))) e) e') (at level 0).
 Definition limpl (l : typ) (e e' : expr typ func) : expr typ func :=
   App (App (Inj (inr (ilf_impl l))) e) e'.
 Definition lor (l : typ) (e e' : expr typ func) : expr typ func :=
@@ -222,9 +320,8 @@ Definition lembed (t f : typ) (e : expr typ func) : expr typ func :=
   App (Inj (inr (ilf_embed f t))) e.
 Definition lnot (t : typ) (e : expr typ func) : expr typ func := limpl t e (lfalse t).
 
-Definition mkeq (t : typ) (e1 e2 : expr typ func) :=
-    App (App (leq t) e1) e2.
-Definition mkneq (t : typ) (e1 e2 : expr typ func) : expr typ func :=
-	lnot tyProp (mkeq t e1 e2).
-	
-
+Definition test_lemma :=
+  @lemmaD typ RType_typ (expr typ func) Expr_expr (expr typ func)
+          (fun tus tvs e => exprD' nil tus tvs tyProp e)
+          tyProp
+          (fun x => x) nil nil.
