MirrorCharge!/src/MirrorCharge/Java/MethodSpecTactics.v
@@ -1,0 +1,218 @@
+Require Import Coq.Strings.String.
+Require Import Coq.PArith.BinPos.
+Require Import ExtLib.Core.RelDec.
+Require Import ExtLib.Data.String.
+Require Import ExtLib.Data.Nat.
+Require Import ExtLib.Data.HList.
+Require Import MirrorCore.Lemma.
+Require Import MirrorCore.TypesI.
+Require Import MirrorCore.Lambda.Expr.
+Require Import MirrorCore.STac.STac.
+Require Import MirrorCore.provers.DefaultProver.
+Require MirrorCore.syms.SymEnv.
+Require MirrorCore.syms.SymSum.
+Require Import MirrorCore.Subst.FMapSubst.
+Require Import MirrorCore.Lambda.ExprLift.
+Require Import MirrorCore.Lambda.ExprSubst.
+Require Import MirrorCore.Lambda.ExprUnify_simul.
+Require Import MirrorCore.Lambda.Red.
+Require Import MirrorCore.Lambda.AppN. 
+Require Import MirrorCharge.ILogicFunc.
+Require Import MirrorCharge.OrderedCanceller.
+Require Import MirrorCharge.BILNormalize.
+Require Import MirrorCharge.SynSepLog.
+Require Import MirrorCharge.SepLogFold.
+
+Require Import MirrorCharge.Java.Syntax.
+
+Require Import Java.Language.Lang.
+Require Import Java.Language.Program.
+
+Require Import Coq.Arith.Peano_dec.
+
+Fixpoint search_NoDup
+    {A} (A_dec: forall a b: A, {a=b}+{a=b->False}) (l: list A) : option (NoDup l) :=
+  match l with
+  | nil => Some (NoDup_nil A)
+  | a::l' =>
+      match search_NoDup A_dec l' with
+      | Some nodup =>
+          match In_dec A_dec a l' with
+          | left isin => None
+          | right notin => 
+ 			match search_NoDup A_dec l' with
+ 				| Some pf => Some (NoDup_cons _ notin pf)
+ 				| None => None         
+            end
+          end
+      | None => None
+      end
+  end.
+
+  Definition list_notin_set lst s :=
+  	fold_right (fun a acc => andb (SS.for_all (fun b => negb (string_dec a b)) s) acc) true lst.
+Print Result.
+
+Definition method_specI : stac typ (expr typ func) subst :=
+  fun tus tvs s lst e =>
+    match e with
+    	| mkEntails [l, mkProgEq [mkProg [P]], mkMethodSpec [C, m, mkVarList [args], r, p, q]] =>
+    	      match C, m with
+    	        | Inj (inl (inr (pString Cname))), Inj (inl (inr (pString Mname))) => 
+    	          match SM.find Cname (p_classes P) with
+    	          	| Some Class => 
+    	          	  match SM.find Mname (c_methods Class) with
+    	          	    | Some Method => 
+						  match search_NoDup Coq.Strings.String.string_dec args with
+						  	| Some pf => 
+						  	  match eq_nat_dec (length args) (length (m_params Method)) with
+						  	    | left pf' => 
+						  	      if list_notin_set args (modifies (m_body Method)) then
+						  	        More tus tvs s lst 
+						  	        mkEntails [l, mkProgEq [mkProg [P]], 
+						  	                      mkTriple [p, mkCmd [m_body Method], q]]
+						  	                      (* Must add substitutions for the arguments here *)
+						  	      else
+						  	        @Fail _ _ _
+						  	    | right _ => @Fail _ _ _
+						  	  end
+						  	| None => @Fail _ _ _
+						  end
+    	          	    | None => @Fail _ _ _
+    	          	  end
+    	          	| None => @Fail _ _ _
+    	          end
+    	        | _, _ => @Fail _ _ _
+    	      end
+      	| _ => @Fail _ _ _
+    end.
+
+Fixpoint tripleE tus tvs (G P Q : expr typ func) l (c : cmd) s args : Result typ (expr typ func) subst :=
+	match c with 
+	  | cskip =>
+	    match @exprUnify subst typ func _ _ RS SS SU 3 nil
+                              tus tvs 0 s P Q tyAsn with
+          | Some s => Solved _ tus tvs s
+          | None   => Fail _ _ _
+        end
+	  | cseq c1 c2 => 
+	    let i := S (length tus) in
+	    match tripleE (tySpec::tus) tvs G P (UVar i) l c1 s args with
+	      | Solved tus tvs s => 
+	        match UVarMap.MAP.find i s with
+	          | Some R => tripleE tus tvs G R Q l c2 s args
+	          | None => Fail _ _ _
+	        end
+	      | _ => More nil nil s args (mkEntails [l, G, mkTriple [P, mkCmd [c], Q]])
+	    end
+	  | _ => More nil nil s args (mkEntails [l, G, mkTriple [P, mkCmd [c], Q]])
+    end.
+    
+
+    
+Definition symE : stac typ (expr typ func) subst :=
+	fun tus tvs s lst e => 
+		match e with 
+			| mkEntails [l, G, mkTriple [P, mkCmd [c], Q]] => 
+			  tripleE tus tvs G P Q l c s lst
+			| _ => Fail _ _ _
+		end.
+
+
+Require Import ExtLib.Tactics.
+Require Import Lambda.ExprTac.
+
+Local Existing Instance SS.
+Local Existing Instance SU.
+Local Existing Instance SO.
+Check @stac_sound.
+
+Lemma symE_sound : @stac_sound typ (expr typ func) subst RType_typ Syntax.Expr_expr _ SS SO symE.
+Proof.
+  intros tus tvs s hs g WFs.
+  remember (symE tus tvs s hs g).
+  
+  destruct r; [apply I | |].
+  unfold symE in Heqr.
+  forward; inv_all; subst.
+
+  unfold goalD; simpl; red_exprD.
+  split; [admit|]. forward.
+  
+  unfold symE in Heqr.
+  forward; inv_all; subst.
+  split; [admit|].
+  unfold goalD. 
+  forward; inv_all; subst.
+  assert (exist t, @exprD' typ RType_typ (expr typ func) Expr_expr (@app typ tus l)
+      (@app typ tvs l0) e (@typ0 typ RType_typ Prop Typ0_Prop) = Some t).
+  assert (exists t, exprD' (tus ++ l) (tvs ++ l0) e (typ0 (F := Prop)) = Some t).
+  simpl in *.
+  induction c; simpl in H15; try (inversion H15; subst). 
+  Check @app_nil_r typ tvs.
+  Check @exprD'_weaken.
+  destruct (@ExprFacts.exprD'_weaken typ RType_typ Typ2_Fun func _ _ _ _ _ _ _ nil tus tvs _ tyProp t nil nil H) as [t' [H3 H4]].
+  simpl in *.
+  simpl in *.
+  rewrite H3.
+  forward_reason.
+  red.
+  unfold ilfunc.
+  rewrite H3.
+  destruct (@ExprFacts.exprD'_weaken typ RType_typ _ (expr typ func) _ _ _ Expr_expr Expr_ok tus tvs _ tyProp t H nil nil) as [t' [H3 H4]].
+  unfold ExprDsimul.ExprDenote.exprD'.
+  SearchAbout exprD' List.app List.nil.
+  pose
+  Check exprD'_weaken.
+  assert ( ExprDsimul.ExprDenote.exprD' nil (tus ++ nil) (tvs ++ nil) tyProp
+      mkEntails  [logic, e3, mkTriple  [e9, mkCmd  [cassign v d], e5]] = Some t).
+  forward_reason.
+  rewrite <- (@app_nil_r typ) in H.
+  replace tvs with (tvs ++ nil) in H by admit.
+  replace(tvs ++ nil) with tvs by (symmetry; apply app_nil_r).
+  rewrite app_nil_r.
+  SearchAbout nil List.app.
+  red_exprD; forward; inv_all; subst.
+  destruct g; inv_all; subst.
+  inversion Heqr; subst. simpl in *. red_exprD.
+  SearchAbout exprD' nth_error_get_hlist_nth.
+  unfold ExprDsimul.ExprDenote.exprD' in H.
+  unfold Open_GetVAs in H. simpl in H. forward; inv_all; subst.
+  red_exprD.
+  progress simpl in *.
+  
+  simpl.
+  
+  forward.
+  red_exprD.  
+  simpl. unfold goalD. simpl.
+  red_exprD. split. admit.
+  forward. split. admit. forward.
+  simp
+  admit.
+Qed.
+  forward.
+  
+  simpl in *.
+  unfold goalD.
+  red_exprD.
+  red_exprD.
+  unfold mk_entails.
+  SearchAbout stac.
+  simpl in *.
+  unfold symE. simpl.
+  forward.
+  forward_reason.
+  unfold symE.
+  forward_reason.
+  destruct g. simpl.
+  remember (goalD tus tvs (Var v)) as g.
+  destruct g; [|tauto]. simpl in *.
+  split; [tauto|].
+  
+  destruct (goalD tus tvs (Var v)); [|tauto].
+  
+  simpl.
+  forward.
+  unfold stac_sound.
+  
